tla-tree/ImmutableDiskTreeHeight.dfy
@@ -1,0 +1,179 @@
+include "ImmutableDiskTreeInv.dfy"
+include "CrashableMap.dfy"
+
+module RefinementProof {
+import opened KVTypes
+import opened ImmutableDiskTree
+import opened ImmutableDiskTreeInv
+import opened MissingLibrary
+import CrashableMap
+
+function NodeAt(k:Constants, table:Table, view:View, addr:int) : Node
+    requires PlausibleDiskSize(k)
+    requires WFTable(k, table)
+    requires AllocatedNbasValid(k, table)
+    requires addr in AllocatedAddresses(k, table)
+    requires FullView(k, view)
+{
+    var nba := table[addr];
+    var lba := LbaForNba(k, nba);
+    var sector := view[lba];
+    sector.node
+}
+
+type Height = Option<int>
+type AddrHeightMap = map<int,int>   // Maps from addresses to height of the tree at that address. Zero is an Unused addr.
+
+predicate LeafNode(node:Node)
+{
+    forall idx :: ValidSlotIndex(node, idx) ==> !node.slots[idx].Pointer?
+}
+
+function HeightForSlot(slot:Slot, heightMap:AddrHeightMap) : (h:Height)
+{
+    match slot {
+        case Empty => Some(1)
+        case Value(datum) => Some(1)
+        case Pointer(idx) => if idx in heightMap then Some(heightMap[idx]) else None
+    }
+}
+
+predicate HeightAtMost(height:Height, bound:int)
+{
+    height.Some? && height.value <= bound
+}
+
+predicate AllSlotHeightsAtMost(node:Node, heightMap:AddrHeightMap, slotCount:int, bound:int)
+{
+    forall i :: 0<=i<slotCount ==> HeightAtMost(HeightForSlot(node.slots[i], heightMap), bound)
+}
+
+function CombineHeights(h1:Height, h2:Height) : Height
+{
+    if h1.Some? && h2.Some?
+    then Some(max(h1.value, h2.value))
+    else None
+}
+
+function {:opaque} DefineHeightNonLeafPrefix(node:Node, heightMap:AddrHeightMap, slotCount:int) : (h:Height)
+    ensures h.Some? ==> AllSlotHeightsAtMost(node, heightMap, slotCount, h.value)
+{
+    if slotCount==0
+    then Some(1)
+    else
+        CombineHeights(
+            DefineHeightNonLeafPrefix(node, heightMap, slotCount-1),
+            HeightForSlot(node.slots[slotCount-1], heightMap))
+}
+
+function DefineHeightAddr(k:Constants, table:Table, view:View, heightMap:AddrHeightMap, addr:int) : (h:Height)
+    ensures h.Some? ==> 0<=h.value
+{
+    if table[addr].Unused?
+    then Some(0)
+    else
+        var node := NodeAt(k, table, view, addr);
+        DefineHeightNonLeafPrefix(node, heightMap, |node.slots|)
+
+}
+
+function {:opaque} SlotHeightMapDef(k:Constants, table:Table, view:View, maxHeight:int) : AddrHeightMap
+{
+    if maxHeight == 0
+    then
+        map addr | addr in ValidAddresses(k) && table[addr].Used? :: 0
+    else
+        map addr | 
+            addr in ValidAddresses(k)
+            && DefineHeightAddr(k, table, view, SlotHeightMapDef(k, table, view, maxHeight-1), addr).Some?
+            :: DefineHeightAddr(k, table, view, SlotHeightMapDef(k, table, view, maxHeight-1), addr).value
+}
+
+function SlotHeightMap(k:Constants, table:Table, view:View) : AddrHeightMap
+{
+    SlotHeightMapDef(k, table, view, k.tableEntries)
+}
+
+// If there are no cycles, then every address can be assigned a height.
+predicate CycleFree(k:Constants, heightMap:AddrHeightMap)
+{
+    heightMap.Keys == ValidAddresses(k)
+}
+
+
+//// left off here
+/*
+
+// The datums at or below slot slotNum of the tree at table[addr].
+function {:opaque} ISlotView(k:Constants, table:Table, view:View, addr:int, slotNum:int) : CrashableMap.View
+{
+    var node := NodeAt(k, table, view, addr);
+    var slot := node[slotNum];
+    match slot {
+        case Empty => CrashableMap.EmptyMap()
+        case Value(datum) => SingletonMap(datum.key, datum.value)
+        case Pointer(idx) => ITreeView(k, table, view, idx, 
+    if slot.Empty
+    then 
+    els
+}
+
+// The datums in the first slotCount slots of the tree at table[addr].
+function {:opaque} ISubtreePrefixView(k:Constants, table:Table, view:View, addr:int, slotCount:int) : CrashableMap.View
+{
+    if slotCount==0
+    then CrashableMap.EmptyMap()
+    else JoinMap(ISubtreeView(k, table, view, addr, slotCount - 1), ISlotView(k, table, view, addr, slotCount - 1))
+}
+
+function ISubtreeView(k:Constants, table:Table, view:View, addr:int) : CrashableMap.View
+{
+    var slotCount := |NodeAt(k, table, view, addr).slots|;
+    ISubtreePrefixView(k, table, view, addr, slotCount)
+}
+
+function ITreeView(k:Constants, table:Table, view:View) : CrashableMap.View
+{
+    ISubtreePrefixView(k, table, view, ROOT_ADDR())
+}
+
+function IEphemeralView(k:Constants, s:Variables) : CrashableMap.View
+{
+    ITreeView(k, s.ephemeralTable, ViewOfCache(s.cache))
+}
+
+function PersistentTable(k:Constants, s:Variables) : Table
+    requires ValidDiskSize(k, s)
+    requires TableBlocksTypeCorrect(k, s)
+{
+    var super := s.disk.sectors[SUPERBLOCK_LBA()];
+    var ti := super.liveTable;
+    var sectors := s.disk.sectors[TableBegin(k, ti) .. TableBegin(k, ti) + k.tableSectors];
+    UnmarshallTable(k, sectors)
+}
+
+function IPersistentView(k:Constants, s:Variables) : CrashableMap.View
+    requires ValidDiskSize(k, s)
+    requires TableBlocksTypeCorrect(k, s)
+    requires AllocatedNbasValid(k, PersistentTable(k, s))
+    requires PersistentAllocatedNodesTypeCorrect(k, s)
+{
+    ITreeView(k, PersistentTable(k, s), ViewOfDisk(s.disk))
+}
+
+function IViews(k:Constants, s:Variables) : seq<CrashableMap.View>
+    requires Inv(k, s)
+{
+    if s.ready?
+    then [IEphemeralView(k, s), IPersistentView(k, s)]
+    else [IPersistentView(k, s)]
+}
+
+function I(k:Constants, s:Variables) : CrashableMap.Variables
+    requires Inv(k, s)
+{
+    CrashableMap.Variables(IViews(k, s))
+}
+*/
+
+} // module
