tla-tree/ImmutableDiskTreeInv.dfy
@@ -1,0 +1,76 @@
+include "ImmutableDiskTree.dfy"
+
+module ImmutableDiskTreeInv {
+import opened KVTypes
+import opened ImmutableDiskTree
+
+predicate SuperblockTypeCorrect(k:Constants, view:View)
+    requires PlausibleDiskSize(k)
+    requires FullView(k, view)
+{
+    && view[0].Superblock?
+}
+
+function PersistentTableIndex(k:Constants, view:View) : TableIndex
+    requires PlausibleDiskSize(k)
+    requires FullView(k, view)
+    requires SuperblockTypeCorrect(k, view)
+{
+    view[0].liveTable
+}
+
+predicate TableBlocksTypeCorrect(k:Constants, view:View)
+    requires PlausibleDiskSize(k)
+    requires FullView(k, view)
+{
+    && SuperblockTypeCorrect(k, view)
+    && TreeDisk.WFTableIndex(PersistentTableIndex(k, view))
+    && forall sectorIdx :: ValidTableSectorIndex(k, sectorIdx) ==>
+        view[TableBegin(k, PersistentTableIndex(k, view)) + sectorIdx].TableSector?
+}
+
+function PersistentTable(k:Constants, view:View) : Table
+    requires PlausibleDiskSize(k)
+    requires FullView(k, view)
+    requires TableBlocksTypeCorrect(k, view)
+{
+    var super := view[SUPERBLOCK_LBA()];
+    var ti := PersistentTableIndex(k, view);
+    var sectors := SubsequenceFromFullView(TableBegin(k, ti), k.tableSectors);
+    UnmarshallTable(k, sectors)
+}
+
+function {:opaque} AllocatedAddresses(k:Constants, table:Table) : (alloced:set<int>)
+    requires WFTable(k, table)
+    ensures forall addr :: addr in alloced <==> addr in ValidAddresses(k) && table[addr].Used?
+{
+    set addr | addr in ValidAddresses(k) && table[addr].Used?
+}
+
+predicate AllocatedNbasValid(k:Constants, table:Table)
+    requires WFTable(k, table)
+{
+    forall addr :: addr in AllocatedAddresses(k, table) ==> ValidNba(k, table[addr])
+}
+
+predicate AllocatedNodeBlocksTypeCorrect(k:Constants, view:View, table:Table)
+    requires PlausibleDiskSize(k)
+    requires FullView(k, view)
+    requires TableBlocksTypeCorrect(k, view)
+    requires WFTable(k, table)
+    requires AllocatedNbasValid(k, table)
+{
+    forall addr :: addr in AllocatedAddresses(k, table) ==> view[LbaForNba(k, table[addr])].NodeSector?
+}
+
+predicate PersistentAllocatedNodesTypeCorrect(k:Constants, view:View)
+    requires PlausibleDiskSize(k)
+    requires FullView(k, view)
+    requires TableBlocksTypeCorrect(k, view)
+    requires AllocatedNbasValid(k, PersistentTable(k, view))
+{
+    AllocatedNodeBlocksTypeCorrect(k, view, PersistentTable(k, view))
+}
+
+
+} // module
